fiat2/src/fiat2/TypeSystem.v
@@ -141,6 +141,10 @@ Inductive type_of_atom : atom -> type -> Prop :=
                type_of_atom (ANone None) (TOption t)
 | TyANone t : type_wf t ->
               type_of_atom (ANone (Some t)) (TOption t)
+| TyAEmptyDict' kt vt : type_wf kt -> type_wf vt ->
+                    type_of_atom (AEmptyDict None) (TDict kt vt)
+| TyAEmptyDict kt vt : type_wf kt -> type_wf vt ->
+                   type_of_atom (AEmptyDict (Some (kt, vt))) (TDict kt vt)
 | TyAUnit : type_of_atom AUnit TUnit.
 
 Inductive type_of_unop : unop -> type -> type -> Prop :=
@@ -180,7 +184,12 @@ Inductive type_of_binop : binop -> type -> type -> type -> Prop :=
 | TyOCons t : type_wf t ->
               type_of_binop OCons t (TList t) (TList t)
 | TyORange : type_of_binop ORange TInt TInt (TList TInt)
-| TyOWRange : type_of_binop OWRange TWord TWord (TList TWord).
+| TyOWRange : type_of_binop OWRange TWord TWord (TList TWord)
+| TyOLookup kt vt : type_of_binop OLookup (TDict kt vt) kt (TOption vt)
+| TyODelete kt vt : type_of_binop ODelete (TDict kt vt) kt (TDict kt vt).
+
+Inductive type_of_ternop : ternop -> type -> type -> type -> type -> Prop :=
+| TyOInsert kt vt : type_of_ternop OInsert (TDict kt vt) kt vt (TDict kt vt).
 
 Section WithMap.
   Context {tenv: map.map string type} {tenv_ok: map.ok tenv}.
@@ -196,6 +205,11 @@ Section WithMap.
                                 type_of Gstore Genv e1 t1 ->
                                 type_of Gstore Genv e2 t2 ->
                                 type_of Gstore Genv (EBinop o e1 e2) t3
+  | TyETernop o e1 e2 e3 t1 t2 t3 t4 : type_of_ternop o t1 t2 t3 t4 ->
+                                       type_of Gstore Genv e1 t1 ->
+                                       type_of Gstore Genv e2 t2 ->
+                                       type_of Gstore Genv e3 t3 ->
+                                       type_of Gstore Genv (ETernop o e1 e2 e3) t4
   | TyEIf e1 e2 e3 t : type_of Gstore Genv e1 TBool ->
                        type_of Gstore Genv e2 t ->
                        type_of Gstore Genv e3 t ->
@@ -220,19 +234,6 @@ Section WithMap.
   | TyEAccess e tl x t : type_of Gstore Genv e (TRecord tl) ->
                          access_record tl x = Success t ->
                          type_of Gstore Genv (EAccess e x) t
-  | TyEDict l kt vt : type_wf kt -> type_wf vt -> (* needed in case l = nil*)
-                      Forall (fun p => type_of Gstore Genv (fst p) kt /\ type_of Gstore Genv (snd p) vt) l ->
-                      type_of Gstore Genv (EDict l) (TDict kt vt)
-  | TyEInsert d kt vt k v : type_of Gstore Genv d (TDict kt vt) ->
-                           type_of Gstore Genv k kt ->
-                           type_of Gstore Genv v vt ->
-                           type_of Gstore Genv (EInsert d k v) (TDict kt vt)
-  | TyEDelete d kt vt k : type_of Gstore Genv d (TDict kt vt) ->
-                           type_of Gstore Genv k kt ->
-                           type_of Gstore Genv (EDelete d k) (TDict kt vt)
-  | TyELookup d kt vt k : type_of Gstore Genv d (TDict kt vt) ->
-                         type_of Gstore Genv k kt ->
-                         type_of Gstore Genv (ELookup d k) (TOption vt)
   | TyEOptMatch e t1 e_none t2 x e_some : type_of Gstore Genv e (TOption t1) ->
                                     type_of Gstore Genv e_none t2 ->
                                     type_of Gstore (map.put Genv x t1) e_some t2 ->
@@ -285,6 +286,11 @@ Section WithMap.
     Hypothesis (f_unop : forall Genv o e t1 t2, type_of_unop o t1 t2 -> type_of Gstore Genv e t1 -> P Genv e t1 -> P Genv (EUnop o e) t2).
     Hypothesis (f_binop : forall Genv o e1 e2 t1 t2 t3, type_of_binop o t1 t2 t3 -> type_of Gstore Genv e1 t1 -> P Genv e1 t1 ->
                                                         type_of Gstore Genv e2 t2 -> P Genv e2 t2 -> P Genv (EBinop o e1 e2) t3).
+    Hypothesis (f_ternop : forall Genv o e1 e2 e3 t1 t2 t3 t4,
+                   type_of_ternop o t1 t2 t3 t4 -> type_of Gstore Genv e1 t1 -> P Genv e1 t1 ->
+                   type_of Gstore Genv e2 t2 -> P Genv e2 t2 ->
+                   type_of Gstore Genv e3 t3 -> P Genv e3 t3 ->
+                   P Genv (ETernop o e1 e2 e3) t4).
     Hypothesis (f_if : forall Genv e1 e2 e3 t, type_of Gstore Genv e1 TBool -> P Genv e1 TBool ->
                                                type_of Gstore Genv e2 t -> P Genv e2 t ->
                                                type_of Gstore Genv e3 t -> P Genv e3 t ->
@@ -310,17 +316,6 @@ Section WithMap.
     Hypothesis (f_access : forall Genv e tl x t, type_of Gstore Genv e (TRecord tl) -> P Genv e (TRecord tl) ->
                                                  access_record tl x = Success t ->
                                                  P Genv (EAccess e x) t).
-    Hypothesis (f_dict : forall Genv l kt vt, type_wf kt -> type_wf vt ->
-                                              Forall (fun p => type_of Gstore Genv (fst p) kt /\ type_of Gstore Genv (snd p) vt) l ->
-                                              Forall (fun p => P Genv (fst p) kt /\ P Genv (snd p) vt) l -> P Genv (EDict l) (TDict kt vt)).
-    Hypothesis (f_insert : forall Genv d kt vt k v, type_of Gstore Genv d (TDict kt vt) -> P Genv d (TDict kt vt) ->
-                                                    type_of Gstore Genv k kt -> P Genv k kt -> type_of Gstore Genv v vt -> P Genv v vt ->
-                                                    P Genv (EInsert d k v) (TDict kt vt)).
-    Hypothesis (f_delete : forall Genv d kt vt k, type_of Gstore Genv d (TDict kt vt) ->
-                                                  P Genv d (TDict kt vt) -> type_of Gstore Genv k kt -> P Genv k kt ->
-                                                  P Genv (EDelete d k) (TDict kt vt)).
-    Hypothesis (f_lookup : forall Genv d kt vt k, type_of Gstore Genv d (TDict kt vt) -> P Genv d (TDict kt vt) ->
-                                                  type_of Gstore Genv k kt -> P Genv k kt -> P Genv (ELookup d k) (TOption vt)).
     Hypothesis (f_optmatch : forall Genv e t1 e_none t2 x e_some, type_of Gstore Genv e (TOption t1) -> P Genv e (TOption t1) ->
                                                                   type_of Gstore Genv e_none t2 -> P Genv e_none t2 ->
                                                                   type_of Gstore (map.put Genv x t1) e_some t2 -> P (map.put Genv x t1) e_some t2 ->
@@ -346,16 +341,6 @@ Section WithMap.
     Section __.
       Context (type_of_IH : forall Genv e t, type_of Gstore Genv e t -> P Genv e t).
 
-      Fixpoint dict_type_of_IH Genv kt vt l (H : Forall (fun p => type_of Gstore Genv (fst p) kt /\ type_of Gstore Genv (snd p) vt) l) : Forall (fun p => P Genv (fst p) kt /\ P Genv (snd p) vt) l :=
-        match H with
-        | Forall_nil _ => Forall_nil _
-        | @Forall_cons _ _ p l Hp Hl =>
-            match Hp with
-            | conj Hfst Hsnd =>
-                @Forall_cons _ _ p l (conj (type_of_IH _ _ _ Hfst) (type_of_IH _ _ _ Hsnd)) (dict_type_of_IH Genv kt vt l Hl)
-            end
-        end.
-
       Fixpoint record_type_of_IH Genv (l : list expr) (tl : list type) (H : Forall2 (type_of Gstore Genv) l tl) : Forall2 (P Genv) l tl :=
         match H with
         | Forall2_nil _ => Forall2_nil _
@@ -370,16 +355,15 @@ Section WithMap.
       | TyEAtom _ _ a t Hatom => f_atom Genv a t Hatom
       | TyEUnop _ _ o e t1 t2 Ho He => f_unop Genv o e t1 t2 Ho He (type_of_IH Genv e t1 He)
       | TyEBinop _ _ o e1 e2 t1 t2 t3 Ho He1 He2 => f_binop Genv o e1 e2 t1 t2 t3 Ho He1 (type_of_IH Genv e1 t1 He1) He2 (type_of_IH Genv e2 t2 He2)
+      | TyETernop _ _ o e1 e2 e3 t1 t2 t3 t4 Ho He1 He2 He3 =>
+          f_ternop Genv o e1 e2 e3 t1 t2 t3 t4 Ho He1 (type_of_IH Genv e1 t1 He1)
+            He2 (type_of_IH Genv e2 t2 He2) He3 (type_of_IH Genv e3 t3 He3)
       | TyEIf _ _ e1 e2 e3 t He1 He2 He3 => f_if Genv e1 e2 e3 t He1 (type_of_IH Genv e1 TBool He1) He2 (type_of_IH Genv e2 t He2) He3 (type_of_IH Genv e3 t He3)
       | TyELet _ _ e1 t1 x e2 t2 He1 He2 => f_let Genv e1 t1 x e2 t2 He1 (type_of_IH Genv e1 t1 He1) He2 (type_of_IH (map.put Genv x t1) e2 t2 He2)
       | TyEFlatmap _ _ e1 t1 x e2 t2 He1 He2 => f_flatmap Genv e1 t1 x e2 t2 He1 (type_of_IH Genv e1 (TList t1) He1) He2 (type_of_IH (map.put Genv x t1) e2 (TList t2) He2)
       | TyEFold _ _ e1 t1 e2 t2 x y e3 He1 He2 He3 => f_fold Genv e1 t1 e2 t2 x y e3 He1 (type_of_IH Genv e1 (TList t1) He1) He2 (type_of_IH Genv e2 t2 He2) He3 (type_of_IH (map.put (map.put Genv x t1) y t2) e3 t2 He3)
       | TyERecord _ _ l tl tl' Hname Hfield Hpermu Hnodup Hsort => f_record Genv l tl tl' Hname Hfield (record_type_of_IH type_of_IH Genv (List.map snd l) (List.map snd tl) Hfield) Hpermu Hnodup Hsort
       | TyEAccess _ _ e tl x t He Hin => f_access Genv e tl x t He (type_of_IH Genv e (TRecord tl) He) Hin
-      | TyEDict _ _ l kt vt Hkt Hvt Hl => f_dict Genv l kt vt Hkt Hvt Hl (dict_type_of_IH type_of_IH Genv kt vt l Hl)
-      | TyEInsert _ _ d kt vt k v Hd Hk Hv => f_insert Genv d kt vt k v Hd (type_of_IH Genv d (TDict kt vt) Hd) Hk (type_of_IH Genv k kt Hk) Hv (type_of_IH Genv v vt Hv)
-      | TyEDelete _ _ d kt vt k Hd Hk => f_delete Genv d kt vt k Hd (type_of_IH Genv d (TDict kt vt) Hd) Hk (type_of_IH Genv k kt Hk)
-      | TyELookup _ _ d kt vt k Hd Hk => f_lookup Genv d kt vt k Hd (type_of_IH Genv d (TDict kt vt) Hd) Hk (type_of_IH Genv k kt Hk)
       | TyEOptMatch _ _ e t1 e_none t2 x e_some He He_none He_some => f_optmatch Genv e t1 e_none t2 x e_some He (type_of_IH Genv e (TOption t1) He) He_none (type_of_IH Genv e_none t2 He_none) He_some (type_of_IH (map.put Genv x t1) e_some t2 He_some)
       | TyEDictFold _ _ d kt vt e0 t k v acc e Hd He0 He => f_dictfold Genv d kt vt e0 t k v acc e Hd (type_of_IH Genv d (TDict kt vt) Hd) He0 (type_of_IH Genv e0 t He0)  He (type_of_IH (map.put (map.put (map.put Genv k kt) v vt) acc t) e t He)
       | TyESort _ _ l t Hl => f_sort Genv l t Hl (type_of_IH Genv l (TList t) Hl)
@@ -417,17 +401,30 @@ Fixpoint type_eqb (t t' : type) {struct t} : bool :=
   | _, _ => false
   end.
 
-Lemma type_eqb_eq : forall t t', type_eqb t t' = true -> t = t'.
+Lemma type_eqb_refl : forall t, type_eqb t t = true.
 Proof.
-  apply (type_IH (fun t => forall t', type_eqb t t' = true -> t = t')); intros;
-    destruct t'; try discriminate; simpl in *; intuition;
-  try (apply H in H0; congruence).
-  - generalize dependent l0. induction l; destruct l0; simpl in *; try discriminate; intuition.
-    destruct (andb (fst a =? fst p)%string (type_eqb (snd a) (snd p))) eqn:E; simpl in *; try discriminate.
-    inversion H; subst. apply (IHl H4) in H0. injection H0; intros; subst.
-    destruct a, p; inversion H; simpl in *; subst. apply andb_prop in E as [EL ER].
-    rewrite eqb_eq in EL. apply H3 in ER. congruence.
-  - apply andb_prop in H1 as [HL HR]. apply H in HL; apply H0 in HR. congruence.
+  induction t using type_IH; auto; cbn.
+  1:{ induction H; try constructor.
+      cbn; rewrite eqb_refl. rewrite IHForall, H; auto. }
+  1:{ rewrite IHt1, IHt2; auto. }
+Qed.
+
+Lemma type_eqb_eq : forall t t', type_eqb t t' = true <-> t = t'.
+Proof.
+  split.
+  1:{ revert t t'.
+      induction t using type_IH; intros;
+        destruct t'; try discriminate; simpl in *; intuition idtac;
+      try (lazymatch goal with
+             IH: context[_ -> _], H: type_eqb _ _ = _ |- _ =>
+               apply IH in H end; congruence).
+      - generalize dependent l0. induction l; destruct l0; simpl in *; try discriminate; intuition.
+        destruct (andb (fst a =? fst p)%string (type_eqb (snd a) (snd p))) eqn:E; simpl in *; try discriminate.
+        inversion H; subst. apply (IHl H4) in H0. injection H0; intros; subst.
+        destruct a, p; inversion H; simpl in *; subst. apply andb_prop in E as [EL ER].
+        rewrite eqb_eq in EL. apply H3 in ER. congruence.
+      - apply andb_prop in H as [HL HR]. apply IHt1 in HL; apply IHt2 in HR. congruence. }
+  1: intro; subst; apply type_eqb_refl.
 Qed.
 
 Definition compare_types (expected : type) (t : type) {A : Type} (a : A): result A :=
@@ -453,6 +450,10 @@ Definition analyze_atom (expected : type) (a : atom) : result atom :=
                         | _ => error:(a "is a list but expected" expected)
                         end
               end
+  | AEmptyDict t => match t with
+                    | Some (kt, vt) => compare_types expected (TDict kt vt) a
+                    | _ => error:(a "is a dictionary but expected" expected)
+                    end
   | AUnit => compare_types expected TUnit a
   end.
 
@@ -475,6 +476,12 @@ Definition synthesize_atom (a : atom) : result (type * atom) :=
                           else error:("Malformed type" t)
               | None => error:("Insufficient type information for" a)
               end
+  | AEmptyDict t => match t with
+                    | Some (kt, vt) => if (type_wf_comp kt && type_wf_comp vt)%bool
+                                       then Success (TDict kt vt, a)
+                                       else error:("Malformed type" kt "or" vt)
+                    | None => error:("Insufficient type information for" a)
+                    end
   | AUnit => Success (TUnit, a)
   end.
 
@@ -537,47 +544,8 @@ Definition get_attr_type (tl : list (string * type)) (s : string) : type :=
   | Failure _ => TUnit
   end.
 
-Fixpoint first_success (l : list (result (type * expr))) :  result type :=
-  match l with
-  | nil => error:("Insufficient type information")
-  | Success (t, e) :: l => Success t
-  | _ :: l => first_success l
-  end.
-
-Fixpoint dict_type_from' (l : list (result (type * expr * type * expr))) : result (type * type * list (expr * expr)) :=
-  match l with
-  | nil => error:("Insufficient type information for dictionary")
-  | Success (kt, ke, vt, ve) :: nil => Success (kt, vt, (ke, ve) :: nil)
-  | Success (kt, ke, vt, ve) :: l => '(kt0, vt0, el) <- dict_type_from' l ;;
-                                     if andb (type_eqb kt kt0) (type_eqb vt vt0) then Success (kt0, vt0, (ke, ve) :: el)
-                                     else error:(ke "has type" kt "and" ve "has type" vt "but expected" kt0 "and" vt0 "respectively")
-  | Failure err :: _ => Failure err
-  end.
-
-Definition dict_type_from (l : list (result (type * expr * type * expr))) : result (type * expr) :=
-  '(kt, vt, el) <- dict_type_from' l ;; Success (TDict kt vt, EDict el).
-
-Fixpoint dict_from' (l : list (result (expr * expr))) : result (list (expr * expr)) :=
-  match l with
-  | nil => Success nil
-  | Success (k, v) :: l => l' <- dict_from' l ;; Success ((k, v) :: l')
-  | Failure err :: _ => Failure err
-  end.
-
-Definition dict_from (l : list (result (expr * expr))) : result expr :=
-  l' <- dict_from' l ;; Success (EDict l').
-
 Section WithMap.
   Context {tenv: map.map string type} {tenv_ok: map.ok tenv}.
-
-    Section __.
-      Context (analyze_expr : tenv -> tenv -> type -> expr -> result expr).
-
-      Definition analyze_dict_body (Gstore Genv : tenv) (kt vt : type) (l : list (expr * expr)) :=
-        dict_from (List.map (fun '(k, v) => k' <- analyze_expr Gstore Genv kt k ;;
-                                            v' <- analyze_expr Gstore Genv vt v ;;
-                                            Success (k', v')) l).
-    End __.
 
   Local Open Scope bool_scope.
   Fixpoint analyze_expr (Gstore Genv : tenv) (expected : type) (e : expr) : result expr :=
@@ -638,6 +606,20 @@ Section WithMap.
                                        end
                             | _ => error:(e "is a boolean but expected" expected)
                             end
+                        | OLookup => '(t1, d') <- synthesize_expr Gstore Genv e1 ;;
+                                     match t1 with
+                                     | TDict kt vt => if type_eqb expected (TOption vt)
+                                                      then k' <- analyze_expr Gstore Genv kt e2 ;;
+                                                           Success (EBinop OLookup d' k')
+                                                      else error:(e "has type" (TOption vt) "but expected" expected)
+                                     | _ => error:(e1 "has type" t1 "but expected a dictionary")
+                                     end
+                        | ODelete => match expected with
+                                     | TDict kt vt => d' <- analyze_expr Gstore Genv (TDict kt vt) e1 ;;
+                                                      k' <- analyze_expr Gstore Genv kt e2 ;;
+                                                      Success (EBinop ODelete d' k')
+                                     | _ => error:(e "is a dictionary but expected" expected)
+                                     end
                         | o => let '(t1, t2, t3) := binop_types o in
                                if type_eqb expected t3
                                then e1' <- analyze_expr Gstore Genv t1 e1 ;;
@@ -645,6 +627,17 @@ Section WithMap.
                                     Success (EBinop o e1' e2')
                                else error:(e "has type" t3 "but expected" expected)
                         end
+    | ETernop o e1 e2 e3 => match o with
+                            | OInsert =>
+                                match expected with
+                                | TDict kt vt =>
+                                    d' <- analyze_expr Gstore Genv (TDict kt vt) e1 ;;
+                                    k' <- analyze_expr Gstore Genv kt e2 ;;
+                                    v' <- analyze_expr Gstore Genv vt e3 ;;
+                                    Success (ETernop OInsert d' k' v')
+                                | _ => error:(e "is a dictionary but expected" expected)
+                                end
+                            end
     | EIf e1 e2 e3 => e1' <- analyze_expr Gstore Genv TBool e1 ;;
                       e2' <- analyze_expr Gstore Genv expected e2 ;;
                       e3' <- analyze_expr Gstore Genv expected e3 ;;
@@ -688,33 +681,6 @@ Section WithMap.
                          t <- access_record l s ;;
                               if type_eqb expected t then Success (EAccess e' s)
                               else error:("Attribute" s "has type" t "but expected" expected)
-                     | t => error:(e "has type" t "but expected a record")
-                     end
-    | EDict l => match expected with
-                 | TDict kt vt => analyze_dict_body analyze_expr Gstore Genv kt vt l
-                 | _ => error:(e "is a dictionary but expected" expected)
-                 end
-    | EInsert d k v => match expected with
-                       | TDict kt vt =>
-                           d' <- analyze_expr Gstore Genv (TDict kt vt) d ;;
-                           k' <- analyze_expr Gstore Genv kt k ;;
-                           v' <- analyze_expr Gstore Genv vt v ;;
-                           Success (EInsert d' k' v')
-                       | _ => error:(e "is a dictionary but expected" expected)
-                       end
-    | EDelete d k => match expected with
-                     | TDict kt vt =>
-                         d' <- analyze_expr Gstore Genv (TDict kt vt) d ;;
-                         k' <- analyze_expr Gstore Genv kt k ;;
-                         Success (EDelete d' k')
-                     | _ => error:(e "is a dictionary but expected" expected)
-                     end
-    | ELookup d k => '(t1, d') <- synthesize_expr Gstore Genv d ;;
-                     match t1 with
-                     | TDict kt vt => if type_eqb expected (TOption vt)
-                                      then k' <- analyze_expr Gstore Genv kt k ;;
-                                           Success (ELookup d' k')
-                                      else error:(e "has type" (TOption vt) "but expected" expected)
                      | t => error:(e "has type" t "but expected a record")
                      end
     | EOptMatch e e_none x e_some =>
@@ -825,11 +791,32 @@ Section WithMap.
                                                   e1' <- analyze_expr Gstore Genv t e1 ;;
                                                   Success (TBool, EBinop o e1' e2')
                                  end
+                             | OLookup => '(t1, d') <- synthesize_expr Gstore Genv e1 ;;
+                                          match t1 with
+                                          | TDict kt vt => k' <- analyze_expr Gstore Genv kt e2 ;;
+                                                           Success (TOption vt, EBinop OLookup d' k')
+                                          | _ => error:(e1 "has type" t1 "but expected a dictionary")
+                                          end
+                             | ODelete => '(t1, d') <- synthesize_expr Gstore Genv e1 ;;
+                                          match t1 with
+                                          | TDict kt _ => k' <- analyze_expr Gstore Genv kt e2 ;;
+                                                          Success (t1, EBinop ODelete d' k')
+                                          | t => error:(e "has type" t "but expected a dictionary")
+                                          end
                              | o => let '(t1, t2, t3) := binop_types o in
                                     e1' <- analyze_expr Gstore Genv t1 e1 ;;
                                     e2' <- analyze_expr Gstore Genv t2 e2 ;;
                                     Success (t3, EBinop o e1' e2')
                              end
+         | ETernop o e1 e2 e3 => match o with
+                                 | OInsert => '(t1, d') <- synthesize_expr Gstore Genv e1 ;;
+                                              match t1 with
+                                              | TDict kt vt => k' <- analyze_expr Gstore Genv kt e2 ;;
+                                                               v' <- analyze_expr Gstore Genv vt e3 ;;
+                                                               Success (t1, ETernop OInsert d' k' v')
+                                              | t => error:(e "has type" t "but expected a dictionary")
+                                              end
+                                 end
          | EIf e1 e2 e3 => e1' <- analyze_expr Gstore Genv TBool e1 ;;
                            match synthesize_expr Gstore Genv e2 with
                            | Success (t, e2') => e3' <- analyze_expr Gstore Genv t e3 ;; Success (t, EIf e1' e2' e3')
@@ -860,31 +847,6 @@ Section WithMap.
                           match t with
                           | TRecord l =>
                               t <- access_record l s ;; Success (t, EAccess e' s)
-                          | t => error:(e "has type" t "but expected a record")
-                          end
-         | EDict l => let kl := List.map (fun '(k, _) => synthesize_expr Gstore Genv k) l in
-                      let vl := List.map (fun '(_, v) => synthesize_expr Gstore Genv v) l in
-                      fst_kt <- first_success kl ;; fst_vt <- first_success vl ;;
-                      d <- analyze_dict_body analyze_expr Gstore Genv fst_kt fst_vt l ;;
-                      Success (TDict fst_kt fst_vt, d)
-
-         | EInsert d k v => '(t1, d') <- synthesize_expr Gstore Genv d ;;
-                            match t1 with
-                            | TDict kt vt => k' <- analyze_expr Gstore Genv kt k ;;
-                                             v' <- analyze_expr Gstore Genv vt v ;;
-                                             Success (t1, EInsert d' k' v')
-                            | t => error:(e "has type" t "but expected a record")
-                            end
-         | EDelete d k => '(t1, d') <- synthesize_expr Gstore Genv d ;;
-                          match t1 with
-                          | TDict kt _ => k' <- analyze_expr Gstore Genv kt k ;;
-                                          Success (t1, EDelete d' k')
-                          | t => error:(e "has type" t "but expected a record")
-                          end
-         | ELookup d k => '(t1, d') <- synthesize_expr Gstore Genv d ;;
-                          match t1 with
-                          | TDict kt vt => k' <- analyze_expr Gstore Genv kt k ;;
-                                           Success (TOption vt, ELookup d' k')
                           | t => error:(e "has type" t "but expected a record")
                           end
          | EOptMatch e e_none x e_some =>
